Thread Semantics.
Still sketchy. Based on meeting with Eliot and Tony plus some subsequent
work on possible monad to be used to abstract and structure
specification. Not sure if we want to just "read" the threadstate (as in
Reader monad), or make it a state monad where we are always allowing for
threadstate transformation.  The memory messages are clearly a Writer
monad (a list of these that accumulates over the bind), and the handling
of errors (Blocked and Abort) is standard.

uvmThreadSemanticsScript.sml
@@ -1,32 +1,156 @@
 open HolKernel Parse boolLib bossLib;
 
 open uvmIRTheory
+open lcsymtacs
+open monadsyntax
 
 val _ = new_theory "uvmThreadSemantics";
 val _ = type_abbrev("tid", ``:num``)
+val _ = type_abbrev("addr", ``:num``)  (* non-local memory addresses *)
 
 
 val _ = Datatype`
   frame = <|
-    function : funcid ;
-    ssavars : SSAVar |-> value
+    function : fnname ;
+    ssavars : SSAVar |-> value option ;
+    code : block_label |-> bblock
   |>`
 
 val _ = Datatype`
-  resumption_point =
-    BlockEntry block_label
-  | BlockExit block_label
+  respt_arg = RPVal value    (* values already computed in resumee's context *)
+            | ResumerArg num (* index into values from resumer *)
 `
 
-val _ = type_abbrev("sus_frame", ``:frame # resumption_point``)
+val _ = type_abbrev(
+  "resumption_point", ``:block_label # respt_arg list``)
+
+val _ = type_abbrev(
+  "respt_pair", ``:resumption_point # resumption_point option``)
+
+val _ = type_abbrev("sus_frame", ``:frame # respt_pair``)
 
 
 val _ = Datatype`
   threadState = <|
     stack : sus_frame list ;
     curframe : frame ;
-    pc : block_label # num ;
-    tid : tid
-|>
+    curblock : block_label ;
+    offset : num ;
+    tid : tid ;
+    memreq_map : num |-> SSAVar
+|>`
+
+val _ = Datatype`
+  memoryMessage = Read addr num (* memreq id *) | Write addr value
+`;
+
+val _ = Datatype`
+  tsstep_result = Success α | Abort | Blocked
+`
+
+val tsresult_case_eq = prove_case_eq_thm {
+  case_def = TypeBase.case_def_of ``:α tsstep_result``,
+  nchotomy = TypeBase.nchotomy_of ``:α tsstep_result``
+};
+
+val paircase_eq = prove(
+  ``(pair_CASE x f = y) ⇔ ∃a b. (x = (a,b)) ∧ (f a b = y)``,
+  Cases_on `x` >> simp[]);
+
+(* set up TSM, a monad *)
+val _ = type_abbrev(
+  "TSM", ``:threadState -> (α # memoryMessage list) tsstep_result``)
+
+val TSUNIT_def = Define`
+  TSUNIT (x:α) :α TSM = λts. Success (x, [])
+`;
+val _ = overload_on ("return", ``TSUNIT``)
+
+val TSBIND_def = Define`
+  TSBIND (x : α TSM) (f : α -> β TSM) : β TSM =
+    λts.
+      case x ts of
+      | Success (a, msgs1) =>
+        (case f a ts of
+         | Success(b, msgs2) => Success(b, msgs1 ++ msgs2)
+         | r => r)
+      | Abort => Abort
+      | Blocked => Blocked
+`;
+
+val TSDIE_def = Define`TSDIE : α TSM = λts. Abort`
+val TSBLOCKED_def = Define`TSBLOCKED : α TSM = λts. Blocked`
+
+val TSBIND_DIEL = store_thm(
+  "TSBIND_DIEL[simp]",
+  ``TSBIND TSDIE f = TSDIE``,
+  simp[FUN_EQ_THM, TSBIND_def, TSDIE_def]);
+
+val TSBIND_UNITL = store_thm(
+  "TSBIND_UNITL[simp]",
+  ``TSBIND (TSUNIT x) f = f x``,
+  dsimp[FUN_EQ_THM, TSBIND_def, TSUNIT_def, tsresult_case_eq, paircase_eq] >>
+  csimp[] >> qx_gen_tac `ts` >> Cases_on `f x ts` >> simp[] >>
+  qcase_tac `f x ts = Success a` >> Cases_on `a` >> simp[]);
+
+val TSBIND_UNITR = store_thm(
+  "TSBIND_UNITR[simp]",
+  ``TSBIND tsm TSUNIT = tsm``,
+  dsimp[FUN_EQ_THM, TSBIND_def, TSUNIT_def, tsresult_case_eq, paircase_eq] >>
+  csimp[] >> qx_gen_tac `ts` >> Cases_on `tsm ts` >> simp[] >>
+  qcase_tac `tsm ts = Success a` >> Cases_on `a` >> simp[]);
+
+val TSGET_def = Define`
+  TSGET : threadState TSM = λts. Success(ts, [])
+`
+
+val readVar_def = Define`
+  readVar (x : SSAVar) : value TSM =
+    do
+      ts <- TSGET ;
+      case FLOOKUP ts.curframe.ssavars x of
+          NONE => TSDIE
+        | SOME NONE => TSBLOCKED
+        | SOME (SOME v) => return v
+    od
+`
+
+val eval_exp_def = Define`
+  eval_exp (e : expression) : (value list) TSM =
+    let cf = ts.curframe in
+      case e of
+        Binop bop v1 v2 =>
+          let val1 = THE (FAPPLY cf.ssavars v1) in
+          let val2 = THE (FAPPLY cf.ssavars v2)
+          in
+            (case evalbop bop val1 val2 of
+                NONE => Abort
+              | SOME result => (result, []))
+      | Load mtype destvar morder =>
+
+
+
+
+'a memory_monad : memoryOp list -> ('a * memoryOp list) option
+
+val exec_inst_def = Define`
+  exec_inst ts0 inst =
+    case inst of
+      Assign vtuple exp =>
+        if ¬expr_ready ts0 exp then Blocked
+        else bind vtuple (eval_exp ts0 exp)
+`
+
+val ts_step_def = Define`
+  ts_step codemap (ts0 : threadState) : tsstep_result =
+    case FLOOKUP ts0.curframe.code ts0.curblock of
+      NONE => Abort
+    | SOME bb =>
+      if ts0.offset > LENGTH bb.body then Abort
+      else if ts0.offset = LENGTH bb.body then exec_terminst ts0 bb.exit
+      else exec_inst ts0 (EL ts0.offset bb.body)
+`;
+
+
 
 val _ = export_theory();
